Bit of progress

experiments/rupicola/Compiler.V3.Correctness.fst
@@ -12,7 +12,7 @@ let rec elab_typ (t:typ) : Type0 = // this could already create universe problem
   | TArr t1 t2 -> (elab_typ t1 -> elab_typ t2)
 
 class compile_typ (s:Type) = {
-  [@@@no_method] t : (t:typ{elab_typ t == s})
+  [@@@no_method] t : (t:typ{elab_typ t == s}) (** CA: is this equality problematic? **)
 }
 
 instance compile_typ_unit : compile_typ unit = { t = TUnit }
@@ -37,7 +37,7 @@ let rec elab_typ_is_compile_typ (t:typ) : compile_typ (elab_typ t) =
     assume (elab_typ t == (elab_typ t1 -> elab_typ t2));
     compile_typ_arrow (elab_typ t1) (elab_typ t2) #(elab_typ_is_compile_typ t1) #(elab_typ_is_compile_typ t2)
 
-let rec inverse_elab_typ_compile_typ (t:typ) : Lemma ((elab_typ_is_compile_typ t).t == t) =
+let rec inverse_elab_typ_compile_typ (t:typ) : Lemma ((elab_typ_is_compile_typ t).t == t) [SMTPat (elab_typ_is_compile_typ t).t] =
   match t with
   | TUnit -> ()
   | TArr t1 t2 ->
@@ -102,31 +102,27 @@ let gsubst (#g:env) #b #g_card (s:gsub g b g_card) (e:exp{fv_in_env g e}) : clos
    It is like a symbol we introduce when dealing with lambdas and eliminate when dealing with variables **)
 
 (** The deBrujin index is inverse to the index in F* env **)
-let var_to_fs (g_card:nat) (x:var{x < g_card}) : (i:nat{i < g_card}) =
-  g_card-x-1
-
-let fs_to_var (g_card:nat) (i:nat{i < g_card}) : var =
-  g_card-i-1
+let var_to_fs (g_card:nat) (x:var{x < g_card}) : (i:nat{i < g_card}) = g_card-x-1
+let fs_to_var (g_card:nat) (i:nat{i < g_card}) : var = g_card-i-1
+let lem_inverse (g_card:nat) (x:var{x < g_card}) : Lemma (fs_to_var g_card (var_to_fs g_card x) == x) = ()
+let lem_inverse' (g_card:nat) (i:var{i < g_card}) : Lemma (var_to_fs g_card (fs_to_var g_card i) == i) = ()
 
 assume type fs_env #g (g_card:env_card g) : Type u#1000 (** having such an env is even possible in practice? what would its universe be? **)
 assume val get_v : #g:_ -> #g_card:env_card g -> fs_env g_card -> i:nat{i < g_card} -> elab_typ (Some?.v (g (fs_to_var g_card i)))
 assume val fs_extend : #g:_ -> #g_card:env_card g -> fs_s:fs_env g_card -> #t:typ -> elab_typ t -> fs_s':(fs_env #(extend t g) (g_card+1))
-assume val fs_pop : #t:typ -> #g:_ -> #g_card:env_card g -> fs_env #(extend t g) (g_card+1) -> fs_env #g g_card
+assume val fs_shrink : #t:typ -> #g:_ -> #g_card:env_card g -> fs_env #(extend t g) (g_card+1) -> fs_env #g g_card
 
 assume val lem_fs_extend #g (#g_card:env_card g) (fs_s:fs_env g_card) #t (v:elab_typ t) : Lemma (
   (forall (i:nat). i < g_card ==> get_v fs_s i == get_v (fs_extend fs_s v) i) /\
   get_v (fs_extend fs_s v) g_card == v)
   [SMTPat (fs_extend fs_s v)]
 
-assume val lem_fs_pop #g (#g_card:env_card g) #t (fs_s:fs_env #(extend t g) (g_card+1)) : Lemma (
-  (forall (i:nat). i < g_card ==> get_v fs_s i == get_v (fs_pop fs_s) i))
-  [SMTPat (fs_pop fs_s)]
+assume val lem_fs_shrink #g (#g_card:env_card g) #t (fs_s:fs_env #(extend t g) (g_card+1)) : Lemma (
+  (forall (i:nat). i < g_card ==> get_v fs_s i == get_v (fs_shrink fs_s) i))
+  [SMTPat (fs_shrink fs_s)]
 
-assume val pop_extend_inverse #g (#g_card:env_card g) (fs_s:fs_env g_card) #t (x:elab_typ t) : Lemma (fs_pop (fs_extend fs_s x) == fs_s)
-  [SMTPat (fs_pop (fs_extend fs_s x))]
-
-let lem_inverse (g_card:nat) (x:var{x < g_card}) : Lemma (fs_to_var g_card (var_to_fs g_card x) == x) = ()
-let lem_inverse' (g_card:nat) (i:var{i < g_card}) : Lemma (var_to_fs g_card (fs_to_var g_card i) == i) = ()
+assume val pop_extend_inverse #g (#g_card:env_card g) (fs_s:fs_env g_card) #t (x:elab_typ t) : Lemma (fs_shrink (fs_extend fs_s x) == fs_s)
+  [SMTPat (fs_shrink (fs_extend fs_s x))]
 
 let (∽) (#g:env) #b #g_card (s:gsub g g_card b) (fs_s:fs_env g_card) : Type0 =
   forall (x:var). Some? (g x) ==>
@@ -153,7 +149,7 @@ let equiv_var #g (g_card:env_card g) (x:var{x < g_card})
   = assert ((fun (fs_s:fs_env g_card) -> get_v fs_s (var_to_fs g_card x)) ≈ EVar x) by (explode ())
 
 let equiv_lam #g (g_card:env_card g) (t1:typ) (body:exp) (t2:typ) (f:fs_env g_card -> elab_typ (TArr t1 t2)) : Lemma
-  (requires (fun fs_s -> f (fs_pop #t1 fs_s) (get_v fs_s g_card)) ≈ body)
+  (requires (fun fs_s -> f (fs_shrink #t1 fs_s) (get_v fs_s g_card)) ≈ body)
             // the asymmetry is here. body is an open expression, while for f, I don't have an open expression
             // the equiv is quantifying over the free variable of body, but not get_v
   (ensures f ≈ (ELam t1 body)) =
@@ -168,13 +164,13 @@ let equiv_lam #g (g_card:env_card g) (t1:typ) (body:exp) (t2:typ) (f:fs_env g_ca
         introduce _ ==> _ with _. begin
           let s' = gsub_extend s t1 v in
           let fs_s' = fs_extend fs_s fs_v in
-          eliminate forall b (s':gsub g' g_card' b) fs_s'. s' ∽ fs_s' ==>  t2 ⋮ (f (fs_pop #t1 fs_s') (get_v fs_s' g_card), (gsubst s' body))
+          eliminate forall b (s':gsub g' g_card' b) fs_s'. s' ∽ fs_s' ==>  t2 ⋮ (f (fs_shrink #t1 fs_s') (get_v fs_s' g_card), (gsubst s' body))
             with false s' fs_s';
           assert (s ∽ fs_s);
           assert (gsub_extend s t1 v ∽ fs_extend fs_s fs_v);
-          assert (t2 ⋮ (f (fs_pop fs_s') (get_v fs_s' g_card), (gsubst s' body)));
+          assert (t2 ⋮ (f (fs_shrink fs_s') (get_v fs_s' g_card), (gsubst s' body)));
           assert (get_v (fs_extend fs_s fs_v) g_card == fs_v);
-          assert (t2 ⋮ (f (fs_pop fs_s') fs_v, (gsubst s' body)));
+          assert (t2 ⋮ (f (fs_shrink fs_s') fs_v, (gsubst s' body)));
           assert (t2 ⋮ (f fs_s fs_v, (gsubst s' body)));
           assume ((subst (sub_beta v) (subst (sub_elam s) body)) == (subst (gsub_extend s t1 v) body)); (** substitution lemma **)
           assert (t2 ⋮ (f fs_s fs_v, subst_beta t1 v body'))
@@ -227,35 +223,73 @@ instance compile_exp_unit g g_card : compile_exp #unit #solve g g_card (fun _ ->
 
 let test_unit g n : compile_exp g n (fun _ -> ()) = solve
 
-instance compile_exp_var (g:env) (g_card:env_card g) (i:nat{i < g_card}) : compile_exp g g_card (fun fs_s -> get_v fs_s i) =
+[@"opaque_to_smt"]
+val get_v' : #g:_ -> #g_card:env_card g -> fs_env g_card -> i:nat{i < g_card} -> a:Type{a == elab_typ (Some?.v (g (fs_to_var g_card i)))} -> a
+let get_v' #g #g_card fs_s i a =
+  get_v #g #g_card fs_s i
+
+instance compile_exp_var (a:Type) {| ca:compile_typ a |} (g:env) (g_card:env_card g) (i:nat{i < g_card /\ ca.t == Some?.v (g (fs_to_var g_card i))})
+  : compile_exp
+      #a
+      #ca
+      g
+      g_card
+      (fun fs_s -> get_v' fs_s i a) =
   let x = fs_to_var g_card i in {
     t = EVar x;
     proof = begin
       inverse_elab_typ_compile_typ (Some?.v (g x));
       TyVar #g x
     end;
-    equiv_proof = (fun () -> equiv_var g_card x);
- }
+    equiv_proof = (fun () ->
+      reveal_opaque (`%get_v') (get_v' #g #g_card);
+      equiv_var g_card x);
+}
 
-instance compile_exp_var3 (g:env) (g_card:env_card g) (t:typ) : compile_exp (extend t g) (g_card+1) (fun fs_s -> get_v fs_s g_card) =
-  let x = fs_to_var (g_card+1) g_card in {
-    t = EVar x;
-    proof = begin
-      inverse_elab_typ_compile_typ (Some?.v ((extend t g) x));
-      TyVar #(extend t g) x
-    end;
-    equiv_proof = (fun () -> equiv_var #(extend t g) (g_card+1) x);
-  }
+let test1_var : compile_exp (extend TUnit empty) 1 (fun fs_s -> get_v' fs_s 0 unit) =
+  solve
 
-instance compile_exp_var2 (g:env) (g_card:env_card g) (t:typ) (i:nat{i < g_card}) : compile_exp (extend t g) (g_card+1) (fun fs_s -> get_v (fs_pop #t fs_s) i) =
+
+//let some_other_lemmas1 (#a:Type) {| ca:compile_typ a |} : Lemma (elab_typ ca.t == a) [SMTPat (elab_typ ca.t)]= ()
+//let some_other_lemmas2 (#a:Type) {| ca:compile_typ a |} : Lemma (elab_typ_is_compile_typ' ca.t == ca) [SMTPat (elab_typ_is_compile_typ' ca.t)] = ()
+
+
+#push-options "--print_implicits"
+
+instance compile_exp_var2 (g:env) (g_card:env_card g) (t:typ) (i:nat{i < g_card}) {| ce:compile_exp (extend t g) (g_card+1) (fun fs_s -> get_v fs_s i) |} : compile_exp (extend t g) (g_card+1) (fun fs_s -> get_v (fs_shrink #t fs_s) i) = {
+  t = ce.t;
+  proof = ce.proof;
+  equiv_proof = (fun () -> ce.equiv_proof ())
+}
+
+instance compile_exp_var2' (a:Type) {| ca:compile_typ a |} (g:env) (g_card:env_card g) (t:typ) (i:nat{i < g_card /\ ca.t == Some?.v ((extend t g) (fs_to_var (g_card+1) i))}) {| ce:compile_exp (extend t g) (g_card+1) (fun fs_s -> get_v' fs_s i a) |} : compile_exp (extend t g) (g_card+1) (fun fs_s -> get_v' (fs_shrink #t fs_s) i a) = {
+  t = ce.t;
+  proof = ce.proof;
+  equiv_proof = (fun () ->
+    admit ();
+      reveal_opaque (`%get_v') (get_v' #g #g_card);
+    ce.equiv_proof ())
+}
+
+(**
+instance compile_exp_var2' (a:Type) {| ca:compile_typ a |} (g:env) (g_card:env_card g) (i:nat{i < g_card /\ ca.t == Some?.v (g (fs_to_var g_card i))}) t
+  : compile_exp
+      #a
+      #ca
+      (extend t g)
+      (g_card+1)
+      (fun fs_s -> get_v' (fs_shrink #t fs_s) i a) =
   let x = fs_to_var (g_card+1) i in {
     t = EVar x;
     proof = begin
       inverse_elab_typ_compile_typ (Some?.v ((extend t g) x));
       TyVar #(extend t g) x
     end;
-    equiv_proof = (fun () -> equiv_var #(extend t g) (g_card+1) x);
-  }
+    equiv_proof = (fun () ->
+      reveal_opaque (`%get_v') (get_v' #g #g_card);
+      equiv_var #(extend t g) (g_card+1) x);
+}**)
+
 
 instance compile_exp_lambda
   g
@@ -263,7 +297,7 @@ instance compile_exp_lambda
   (#a:Type) {| ca: compile_typ a |}
   (#b:Type) {| cb: compile_typ b |}
   (f:fs_env g_card -> a -> b)
-  {| cf: compile_exp #b #cb (extend ca.t g) (g_card+1) (fun fs_s -> f (fs_pop #ca.t fs_s) (get_v fs_s g_card)) |}
+  {| cf: compile_exp #b #cb (extend ca.t g) (g_card+1) (fun fs_s -> f (fs_shrink #ca.t fs_s) (get_v' fs_s g_card a)) |}
   : compile_exp #_ #(compile_typ_arrow a b) g g_card (fun (fs_s:fs_env g_card) -> f fs_s) = {
   t = begin
     let g' = extend ca.t g in
@@ -274,6 +308,7 @@ instance compile_exp_lambda
   proof = TyLam #g ca.t cf.proof;
   equiv_proof = (fun () ->
     cf.equiv_proof ();
+    reveal_opaque (`%get_v') (get_v' #(extend ca.t g) #(g_card+1));
     equiv_lam g_card ca.t cf.t cb.t f
   )
 }
@@ -287,22 +322,29 @@ let test1_exp : compile_whole #(unit -> unit) (fun x -> ()) =
 let _ = assert (test1_exp.t == ELam TUnit (EUnit))
 
 let test2_exp : compile_whole #(unit -> unit) (fun x -> x) =
-  compile_exp_lambda empty 0 (fun _ x -> x)
-    #(compile_exp_var3 empty 0 compile_typ_unit.t)
-    //#(compile_exp_var (extend compile_typ_unit.t empty) 1 0)
+  solve
 let _ = assert (test2_exp.t == ELam TUnit (EVar 0))
 
 let test3_exp : compile_whole #(unit -> unit -> unit) (fun x y -> x) =
   compile_exp_lambda empty 0 (fun _ x y -> x) (** CA: returning y instead of x does not return any error! **)
-    #(compile_exp_lambda (extend TUnit empty) 1 (fun fs_s y -> get_v fs_s 0)
-      #(compile_exp_var2 (extend TUnit empty) 1 TUnit 0))
+    #(compile_exp_lambda (extend TUnit empty) 1 (fun fs_s y -> get_v' fs_s 0 unit)
+      #(compile_exp_var2' unit (extend TUnit empty) 1 TUnit 0 #solve))
+
+(**
+[@expect_failure]
+let test3_exp3 : compile_whole #(unit -> unit -> unit) (fun x y -> x) =
+  compile_exp_lambda empty 0 (fun _ x y -> y) (** CA: returning y instead of x does not return any error! **)
+    #(compile_exp_lambda (extend TUnit empty) 1 (fun fs_s y -> get_v' fs_s 0 unit)
+      #(compile_exp_var2' unit (extend TUnit empty) 1 TUnit 0 #solve))
+**)
 
 let _ = assert (test3_exp.t == ELam TUnit (ELam TUnit (EVar 1)))
 
 let test4_exp : compile_whole #(unit -> unit -> unit) (fun x y -> y) =
   compile_exp_lambda empty 0 (fun _ x y -> y)
     #(compile_exp_lambda (extend TUnit empty) 1 (fun fs_s y -> y)
-      #(compile_exp_var (extend TUnit (extend TUnit empty)) 2 1))
+      #(compile_exp_var unit (extend TUnit (extend TUnit empty)) 2 1))
+
 let _ = assert (test4_exp.t == ELam TUnit (ELam TUnit (EVar 0)))
 
 instance compile_exp_app
